commit

build1/ir/Src/Prover/Set.c
@@ -1,0 +1,1605 @@
+// Lean compiler output
+// Module: Src.Prover.Set
+// Imports: Init Src.Prover.Choice
+#include <lean/lean.h>
+#if defined(__clang__)
+#pragma clang diagnostic ignored "-Wunused-parameter"
+#pragma clang diagnostic ignored "-Wunused-label"
+#elif defined(__GNUC__) && !defined(__CLANG__)
+#pragma GCC diagnostic ignored "-Wunused-parameter"
+#pragma GCC diagnostic ignored "-Wunused-label"
+#pragma GCC diagnostic ignored "-Wunused-but-set-variable"
+#endif
+#ifdef __cplusplus
+extern "C" {
+#endif
+static lean_object* l_prover___aux__Src__Prover__Set______macroRules__prover__term___u2208____1___closed__10;
+lean_object* lean_mk_empty_array_with_capacity(lean_object*);
+extern lean_object* l_Lean_nullKind;
+lean_object* lean_name_mk_string(lean_object*, lean_object*);
+static lean_object* l_prover___aux__Src__Prover__Set______macroRules__prover__term___u2286____1___closed__6;
+static lean_object* l_prover___aux__Src__Prover__Set______macroRules__prover__term___u2208____1___closed__16;
+static lean_object* l_prover___aux__Src__Prover__Set______unexpand__prover__mem__1___closed__2;
+static lean_object* l_prover_term___u2208_____closed__3;
+static lean_object* l_prover_term___u2208_____closed__6;
+lean_object* l_Lean_MonadRef_mkInfoFromRefPos___at___aux__Init__Notation______macroRules__precMax__1___spec__1(lean_object*, lean_object*);
+LEAN_EXPORT lean_object* l_prover___aux__Src__Prover__Set______unexpand__prover__mem__1___boxed(lean_object*, lean_object*, lean_object*);
+lean_object* lean_array_push(lean_object*, lean_object*);
+static lean_object* l_prover___aux__Src__Prover__Set______unexpand__prover__mem__1___closed__1;
+static lean_object* l_prover___aux__Src__Prover__Set______unexpand__prover__mem__1___closed__3;
+static lean_object* l_prover___aux__Src__Prover__Set______macroRules__prover__term___u2209____1___closed__7;
+static lean_object* l_prover___aux__Src__Prover__Set______macroRules__prover__term___u2286____1___closed__2;
+LEAN_EXPORT lean_object* l_prover_term___u2208__;
+lean_object* lean_string_utf8_byte_size(lean_object*);
+static lean_object* l_prover_term___u2208_____closed__5;
+LEAN_EXPORT lean_object* l_prover___aux__Src__Prover__Set______macroRules__prover__term___u2208____1(lean_object*, lean_object*, lean_object*);
+static lean_object* l_prover___aux__Src__Prover__Set______macroRules__prover__term___u2208____1___closed__5;
+static lean_object* l_prover___aux__Src__Prover__Set______macroRules__prover__term___u2208____1___closed__14;
+static lean_object* l_prover_term___u2208_____closed__1;
+static lean_object* l_prover___aux__Src__Prover__Set______macroRules__prover__term___u2209____1___closed__5;
+static lean_object* l_prover___aux__Src__Prover__Set______macroRules__prover__term___u2209____1___closed__3;
+static lean_object* l_prover___aux__Src__Prover__Set______macroRules__prover__term___u2209____1___closed__2;
+static lean_object* l_prover_term___u2208_____closed__4;
+static lean_object* l_prover_term___u2208_____closed__8;
+lean_object* l_Lean_MonadRef_mkInfoFromRefPos___at___aux__Init__Notation______unexpand__Function__comp__1___spec__1(lean_object*, lean_object*);
+static lean_object* l_prover___aux__Src__Prover__Set______macroRules__prover__term___u2286____1___closed__1;
+static lean_object* l_prover_term___u2208_____closed__9;
+static lean_object* l_prover___aux__Src__Prover__Set______macroRules__prover__term___u2208____1___closed__7;
+static lean_object* l_prover_term___u2208_____closed__13;
+static lean_object* l_prover___aux__Src__Prover__Set______macroRules__prover__term___u2286____1___closed__4;
+lean_object* l_Lean_replaceRef(lean_object*, lean_object*);
+static lean_object* l_prover_term___u2286_____closed__1;
+static lean_object* l_prover_term___u2286_____closed__4;
+LEAN_EXPORT lean_object* l_prover___aux__Src__Prover__Set______unexpand__prover__not__mem__1(lean_object*, lean_object*, lean_object*);
+static lean_object* l_prover___aux__Src__Prover__Set______macroRules__prover__term___u2209____1___closed__6;
+static lean_object* l_prover_term___u2286_____closed__2;
+static lean_object* l_prover___aux__Src__Prover__Set______macroRules__prover__term___u2286____1___closed__3;
+static lean_object* l_prover___aux__Src__Prover__Set______macroRules__prover__term___u2286____1___closed__5;
+static lean_object* l_prover_term___u2208_____closed__10;
+static lean_object* l_prover___aux__Src__Prover__Set______macroRules__prover__term___u2208____1___closed__3;
+static lean_object* l_prover___aux__Src__Prover__Set______macroRules__prover__term___u2208____1___closed__15;
+static lean_object* l_prover___aux__Src__Prover__Set______macroRules__prover__term___u2208____1___closed__18;
+static lean_object* l_prover_term___u2209_____closed__5;
+static lean_object* l_prover_term___u2286_____closed__3;
+static lean_object* l_prover_term___u2286_____closed__5;
+static lean_object* l_prover___aux__Src__Prover__Set______macroRules__prover__term___u2208____1___closed__2;
+static lean_object* l_prover_term___u2209_____closed__3;
+static lean_object* l_prover___aux__Src__Prover__Set______macroRules__prover__term___u2208____1___closed__1;
+static lean_object* l_prover___aux__Src__Prover__Set______macroRules__prover__term___u2209____1___closed__1;
+static lean_object* l_prover_term___u2208_____closed__12;
+lean_object* l_Lean_addMacroScope(lean_object*, lean_object*, lean_object*);
+static lean_object* l_prover___aux__Src__Prover__Set______macroRules__prover__term___u2208____1___closed__8;
+static lean_object* l_prover___aux__Src__Prover__Set______macroRules__prover__term___u2208____1___closed__17;
+uint8_t l_Lean_Syntax_isNodeOf(lean_object*, lean_object*, lean_object*);
+static lean_object* l_prover___aux__Src__Prover__Set______macroRules__prover__term___u2208____1___closed__4;
+static lean_object* l_prover___aux__Src__Prover__Set______macroRules__prover__term___u2208____1___closed__6;
+LEAN_EXPORT lean_object* l_prover_term___u2209__;
+static lean_object* l_prover_term___u2286_____closed__6;
+LEAN_EXPORT lean_object* l_prover___aux__Src__Prover__Set______unexpand__prover__subset__1(lean_object*, lean_object*, lean_object*);
+LEAN_EXPORT lean_object* l_prover_term___u2286__;
+LEAN_EXPORT lean_object* l_prover___aux__Src__Prover__Set______unexpand__prover__mem__1(lean_object*, lean_object*, lean_object*);
+static lean_object* l_prover___aux__Src__Prover__Set______macroRules__prover__term___u2208____1___closed__13;
+LEAN_EXPORT lean_object* l_prover___aux__Src__Prover__Set______unexpand__prover__not__mem__1___boxed(lean_object*, lean_object*, lean_object*);
+static lean_object* l_prover_term___u2208_____closed__11;
+static lean_object* l_prover___aux__Src__Prover__Set______macroRules__prover__term___u2208____1___closed__11;
+LEAN_EXPORT lean_object* l_prover___aux__Src__Prover__Set______unexpand__prover__subset__1___boxed(lean_object*, lean_object*, lean_object*);
+uint8_t l_Lean_Syntax_isOfKind(lean_object*, lean_object*);
+static lean_object* l_prover___aux__Src__Prover__Set______macroRules__prover__term___u2286____1___closed__7;
+static lean_object* l_prover_term___u2209_____closed__6;
+LEAN_EXPORT lean_object* l_prover___aux__Src__Prover__Set______macroRules__prover__term___u2286____1(lean_object*, lean_object*, lean_object*);
+static lean_object* l_prover_term___u2209_____closed__4;
+lean_object* l_Lean_Syntax_getArg(lean_object*, lean_object*);
+static lean_object* l_prover___aux__Src__Prover__Set______macroRules__prover__term___u2208____1___closed__12;
+static lean_object* l_prover___aux__Src__Prover__Set______macroRules__prover__term___u2208____1___closed__9;
+static lean_object* l_prover___aux__Src__Prover__Set______macroRules__prover__term___u2209____1___closed__4;
+static lean_object* l_prover_term___u2209_____closed__1;
+static lean_object* l_prover_term___u2208_____closed__7;
+LEAN_EXPORT lean_object* l_prover___aux__Src__Prover__Set______macroRules__prover__term___u2209____1(lean_object*, lean_object*, lean_object*);
+static lean_object* l_prover_term___u2208_____closed__2;
+static lean_object* l_prover_term___u2209_____closed__2;
+static lean_object* _init_l_prover_term___u2208_____closed__1() {
+_start:
+{
+lean_object* x_1; 
+x_1 = lean_mk_string_from_bytes("prover", 6);
+return x_1;
+}
+}
+static lean_object* _init_l_prover_term___u2208_____closed__2() {
+_start:
+{
+lean_object* x_1; lean_object* x_2; lean_object* x_3; 
+x_1 = lean_box(0);
+x_2 = l_prover_term___u2208_____closed__1;
+x_3 = lean_name_mk_string(x_1, x_2);
+return x_3;
+}
+}
+static lean_object* _init_l_prover_term___u2208_____closed__3() {
+_start:
+{
+lean_object* x_1; 
+x_1 = lean_mk_string_from_bytes("term_∈_", 9);
+return x_1;
+}
+}
+static lean_object* _init_l_prover_term___u2208_____closed__4() {
+_start:
+{
+lean_object* x_1; lean_object* x_2; lean_object* x_3; 
+x_1 = l_prover_term___u2208_____closed__2;
+x_2 = l_prover_term___u2208_____closed__3;
+x_3 = lean_name_mk_string(x_1, x_2);
+return x_3;
+}
+}
+static lean_object* _init_l_prover_term___u2208_____closed__5() {
+_start:
+{
+lean_object* x_1; 
+x_1 = lean_mk_string_from_bytes("andthen", 7);
+return x_1;
+}
+}
+static lean_object* _init_l_prover_term___u2208_____closed__6() {
+_start:
+{
+lean_object* x_1; lean_object* x_2; lean_object* x_3; 
+x_1 = lean_box(0);
+x_2 = l_prover_term___u2208_____closed__5;
+x_3 = lean_name_mk_string(x_1, x_2);
+return x_3;
+}
+}
+static lean_object* _init_l_prover_term___u2208_____closed__7() {
+_start:
+{
+lean_object* x_1; 
+x_1 = lean_mk_string_from_bytes(" ∈ ", 5);
+return x_1;
+}
+}
+static lean_object* _init_l_prover_term___u2208_____closed__8() {
+_start:
+{
+lean_object* x_1; lean_object* x_2; 
+x_1 = l_prover_term___u2208_____closed__7;
+x_2 = lean_alloc_ctor(5, 1, 0);
+lean_ctor_set(x_2, 0, x_1);
+return x_2;
+}
+}
+static lean_object* _init_l_prover_term___u2208_____closed__9() {
+_start:
+{
+lean_object* x_1; 
+x_1 = lean_mk_string_from_bytes("term", 4);
+return x_1;
+}
+}
+static lean_object* _init_l_prover_term___u2208_____closed__10() {
+_start:
+{
+lean_object* x_1; lean_object* x_2; lean_object* x_3; 
+x_1 = lean_box(0);
+x_2 = l_prover_term___u2208_____closed__9;
+x_3 = lean_name_mk_string(x_1, x_2);
+return x_3;
+}
+}
+static lean_object* _init_l_prover_term___u2208_____closed__11() {
+_start:
+{
+lean_object* x_1; lean_object* x_2; lean_object* x_3; 
+x_1 = l_prover_term___u2208_____closed__10;
+x_2 = lean_unsigned_to_nat(51u);
+x_3 = lean_alloc_ctor(7, 2, 0);
+lean_ctor_set(x_3, 0, x_1);
+lean_ctor_set(x_3, 1, x_2);
+return x_3;
+}
+}
+static lean_object* _init_l_prover_term___u2208_____closed__12() {
+_start:
+{
+lean_object* x_1; lean_object* x_2; lean_object* x_3; lean_object* x_4; 
+x_1 = l_prover_term___u2208_____closed__6;
+x_2 = l_prover_term___u2208_____closed__8;
+x_3 = l_prover_term___u2208_____closed__11;
+x_4 = lean_alloc_ctor(2, 3, 0);
+lean_ctor_set(x_4, 0, x_1);
+lean_ctor_set(x_4, 1, x_2);
+lean_ctor_set(x_4, 2, x_3);
+return x_4;
+}
+}
+static lean_object* _init_l_prover_term___u2208_____closed__13() {
+_start:
+{
+lean_object* x_1; lean_object* x_2; lean_object* x_3; lean_object* x_4; lean_object* x_5; 
+x_1 = l_prover_term___u2208_____closed__4;
+x_2 = lean_unsigned_to_nat(50u);
+x_3 = lean_unsigned_to_nat(51u);
+x_4 = l_prover_term___u2208_____closed__12;
+x_5 = lean_alloc_ctor(4, 4, 0);
+lean_ctor_set(x_5, 0, x_1);
+lean_ctor_set(x_5, 1, x_2);
+lean_ctor_set(x_5, 2, x_3);
+lean_ctor_set(x_5, 3, x_4);
+return x_5;
+}
+}
+static lean_object* _init_l_prover_term___u2208__() {
+_start:
+{
+lean_object* x_1; 
+x_1 = l_prover_term___u2208_____closed__13;
+return x_1;
+}
+}
+static lean_object* _init_l_prover___aux__Src__Prover__Set______macroRules__prover__term___u2208____1___closed__1() {
+_start:
+{
+lean_object* x_1; 
+x_1 = lean_mk_string_from_bytes("Lean", 4);
+return x_1;
+}
+}
+static lean_object* _init_l_prover___aux__Src__Prover__Set______macroRules__prover__term___u2208____1___closed__2() {
+_start:
+{
+lean_object* x_1; lean_object* x_2; lean_object* x_3; 
+x_1 = lean_box(0);
+x_2 = l_prover___aux__Src__Prover__Set______macroRules__prover__term___u2208____1___closed__1;
+x_3 = lean_name_mk_string(x_1, x_2);
+return x_3;
+}
+}
+static lean_object* _init_l_prover___aux__Src__Prover__Set______macroRules__prover__term___u2208____1___closed__3() {
+_start:
+{
+lean_object* x_1; 
+x_1 = lean_mk_string_from_bytes("Parser", 6);
+return x_1;
+}
+}
+static lean_object* _init_l_prover___aux__Src__Prover__Set______macroRules__prover__term___u2208____1___closed__4() {
+_start:
+{
+lean_object* x_1; lean_object* x_2; lean_object* x_3; 
+x_1 = l_prover___aux__Src__Prover__Set______macroRules__prover__term___u2208____1___closed__2;
+x_2 = l_prover___aux__Src__Prover__Set______macroRules__prover__term___u2208____1___closed__3;
+x_3 = lean_name_mk_string(x_1, x_2);
+return x_3;
+}
+}
+static lean_object* _init_l_prover___aux__Src__Prover__Set______macroRules__prover__term___u2208____1___closed__5() {
+_start:
+{
+lean_object* x_1; 
+x_1 = lean_mk_string_from_bytes("Term", 4);
+return x_1;
+}
+}
+static lean_object* _init_l_prover___aux__Src__Prover__Set______macroRules__prover__term___u2208____1___closed__6() {
+_start:
+{
+lean_object* x_1; lean_object* x_2; lean_object* x_3; 
+x_1 = l_prover___aux__Src__Prover__Set______macroRules__prover__term___u2208____1___closed__4;
+x_2 = l_prover___aux__Src__Prover__Set______macroRules__prover__term___u2208____1___closed__5;
+x_3 = lean_name_mk_string(x_1, x_2);
+return x_3;
+}
+}
+static lean_object* _init_l_prover___aux__Src__Prover__Set______macroRules__prover__term___u2208____1___closed__7() {
+_start:
+{
+lean_object* x_1; 
+x_1 = lean_mk_string_from_bytes("app", 3);
+return x_1;
+}
+}
+static lean_object* _init_l_prover___aux__Src__Prover__Set______macroRules__prover__term___u2208____1___closed__8() {
+_start:
+{
+lean_object* x_1; lean_object* x_2; lean_object* x_3; 
+x_1 = l_prover___aux__Src__Prover__Set______macroRules__prover__term___u2208____1___closed__6;
+x_2 = l_prover___aux__Src__Prover__Set______macroRules__prover__term___u2208____1___closed__7;
+x_3 = lean_name_mk_string(x_1, x_2);
+return x_3;
+}
+}
+static lean_object* _init_l_prover___aux__Src__Prover__Set______macroRules__prover__term___u2208____1___closed__9() {
+_start:
+{
+lean_object* x_1; 
+x_1 = lean_mk_string_from_bytes("mem", 3);
+return x_1;
+}
+}
+static lean_object* _init_l_prover___aux__Src__Prover__Set______macroRules__prover__term___u2208____1___closed__10() {
+_start:
+{
+lean_object* x_1; lean_object* x_2; 
+x_1 = l_prover___aux__Src__Prover__Set______macroRules__prover__term___u2208____1___closed__9;
+x_2 = lean_string_utf8_byte_size(x_1);
+return x_2;
+}
+}
+static lean_object* _init_l_prover___aux__Src__Prover__Set______macroRules__prover__term___u2208____1___closed__11() {
+_start:
+{
+lean_object* x_1; lean_object* x_2; lean_object* x_3; lean_object* x_4; 
+x_1 = l_prover___aux__Src__Prover__Set______macroRules__prover__term___u2208____1___closed__9;
+x_2 = lean_unsigned_to_nat(0u);
+x_3 = l_prover___aux__Src__Prover__Set______macroRules__prover__term___u2208____1___closed__10;
+x_4 = lean_alloc_ctor(0, 3, 0);
+lean_ctor_set(x_4, 0, x_1);
+lean_ctor_set(x_4, 1, x_2);
+lean_ctor_set(x_4, 2, x_3);
+return x_4;
+}
+}
+static lean_object* _init_l_prover___aux__Src__Prover__Set______macroRules__prover__term___u2208____1___closed__12() {
+_start:
+{
+lean_object* x_1; lean_object* x_2; lean_object* x_3; 
+x_1 = lean_box(0);
+x_2 = l_prover___aux__Src__Prover__Set______macroRules__prover__term___u2208____1___closed__9;
+x_3 = lean_name_mk_string(x_1, x_2);
+return x_3;
+}
+}
+static lean_object* _init_l_prover___aux__Src__Prover__Set______macroRules__prover__term___u2208____1___closed__13() {
+_start:
+{
+lean_object* x_1; lean_object* x_2; lean_object* x_3; 
+x_1 = l_prover_term___u2208_____closed__2;
+x_2 = l_prover___aux__Src__Prover__Set______macroRules__prover__term___u2208____1___closed__9;
+x_3 = lean_name_mk_string(x_1, x_2);
+return x_3;
+}
+}
+static lean_object* _init_l_prover___aux__Src__Prover__Set______macroRules__prover__term___u2208____1___closed__14() {
+_start:
+{
+lean_object* x_1; lean_object* x_2; lean_object* x_3; 
+x_1 = lean_box(0);
+x_2 = l_prover___aux__Src__Prover__Set______macroRules__prover__term___u2208____1___closed__13;
+x_3 = lean_alloc_ctor(0, 2, 0);
+lean_ctor_set(x_3, 0, x_2);
+lean_ctor_set(x_3, 1, x_1);
+return x_3;
+}
+}
+static lean_object* _init_l_prover___aux__Src__Prover__Set______macroRules__prover__term___u2208____1___closed__15() {
+_start:
+{
+lean_object* x_1; lean_object* x_2; lean_object* x_3; 
+x_1 = lean_box(0);
+x_2 = l_prover___aux__Src__Prover__Set______macroRules__prover__term___u2208____1___closed__14;
+x_3 = lean_alloc_ctor(1, 2, 0);
+lean_ctor_set(x_3, 0, x_2);
+lean_ctor_set(x_3, 1, x_1);
+return x_3;
+}
+}
+static lean_object* _init_l_prover___aux__Src__Prover__Set______macroRules__prover__term___u2208____1___closed__16() {
+_start:
+{
+lean_object* x_1; 
+x_1 = lean_mk_string_from_bytes("null", 4);
+return x_1;
+}
+}
+static lean_object* _init_l_prover___aux__Src__Prover__Set______macroRules__prover__term___u2208____1___closed__17() {
+_start:
+{
+lean_object* x_1; lean_object* x_2; lean_object* x_3; 
+x_1 = lean_box(0);
+x_2 = l_prover___aux__Src__Prover__Set______macroRules__prover__term___u2208____1___closed__16;
+x_3 = lean_name_mk_string(x_1, x_2);
+return x_3;
+}
+}
+static lean_object* _init_l_prover___aux__Src__Prover__Set______macroRules__prover__term___u2208____1___closed__18() {
+_start:
+{
+lean_object* x_1; lean_object* x_2; 
+x_1 = lean_unsigned_to_nat(2u);
+x_2 = lean_mk_empty_array_with_capacity(x_1);
+return x_2;
+}
+}
+LEAN_EXPORT lean_object* l_prover___aux__Src__Prover__Set______macroRules__prover__term___u2208____1(lean_object* x_1, lean_object* x_2, lean_object* x_3) {
+_start:
+{
+lean_object* x_4; uint8_t x_5; 
+x_4 = l_prover_term___u2208_____closed__4;
+lean_inc(x_1);
+x_5 = l_Lean_Syntax_isOfKind(x_1, x_4);
+if (x_5 == 0)
+{
+lean_object* x_6; lean_object* x_7; 
+lean_dec(x_2);
+lean_dec(x_1);
+x_6 = lean_box(1);
+x_7 = lean_alloc_ctor(1, 2, 0);
+lean_ctor_set(x_7, 0, x_6);
+lean_ctor_set(x_7, 1, x_3);
+return x_7;
+}
+else
+{
+lean_object* x_8; lean_object* x_9; lean_object* x_10; lean_object* x_11; lean_object* x_12; uint8_t x_13; 
+x_8 = lean_unsigned_to_nat(0u);
+x_9 = l_Lean_Syntax_getArg(x_1, x_8);
+x_10 = lean_unsigned_to_nat(2u);
+x_11 = l_Lean_Syntax_getArg(x_1, x_10);
+lean_dec(x_1);
+lean_inc(x_2);
+x_12 = l_Lean_MonadRef_mkInfoFromRefPos___at___aux__Init__Notation______macroRules__precMax__1___spec__1(x_2, x_3);
+x_13 = !lean_is_exclusive(x_12);
+if (x_13 == 0)
+{
+lean_object* x_14; lean_object* x_15; lean_object* x_16; lean_object* x_17; lean_object* x_18; lean_object* x_19; lean_object* x_20; lean_object* x_21; lean_object* x_22; lean_object* x_23; lean_object* x_24; lean_object* x_25; lean_object* x_26; lean_object* x_27; lean_object* x_28; lean_object* x_29; lean_object* x_30; lean_object* x_31; 
+x_14 = lean_ctor_get(x_12, 0);
+x_15 = lean_ctor_get(x_2, 2);
+lean_inc(x_15);
+x_16 = lean_ctor_get(x_2, 1);
+lean_inc(x_16);
+lean_dec(x_2);
+x_17 = l_prover___aux__Src__Prover__Set______macroRules__prover__term___u2208____1___closed__12;
+x_18 = l_Lean_addMacroScope(x_16, x_17, x_15);
+x_19 = l_prover___aux__Src__Prover__Set______macroRules__prover__term___u2208____1___closed__11;
+x_20 = l_prover___aux__Src__Prover__Set______macroRules__prover__term___u2208____1___closed__15;
+x_21 = lean_alloc_ctor(3, 4, 0);
+lean_ctor_set(x_21, 0, x_14);
+lean_ctor_set(x_21, 1, x_19);
+lean_ctor_set(x_21, 2, x_18);
+lean_ctor_set(x_21, 3, x_20);
+x_22 = l_prover___aux__Src__Prover__Set______macroRules__prover__term___u2208____1___closed__18;
+x_23 = lean_array_push(x_22, x_9);
+x_24 = lean_array_push(x_23, x_11);
+x_25 = lean_box(2);
+x_26 = l_prover___aux__Src__Prover__Set______macroRules__prover__term___u2208____1___closed__17;
+x_27 = lean_alloc_ctor(1, 3, 0);
+lean_ctor_set(x_27, 0, x_25);
+lean_ctor_set(x_27, 1, x_26);
+lean_ctor_set(x_27, 2, x_24);
+x_28 = lean_array_push(x_22, x_21);
+x_29 = lean_array_push(x_28, x_27);
+x_30 = l_prover___aux__Src__Prover__Set______macroRules__prover__term___u2208____1___closed__8;
+x_31 = lean_alloc_ctor(1, 3, 0);
+lean_ctor_set(x_31, 0, x_25);
+lean_ctor_set(x_31, 1, x_30);
+lean_ctor_set(x_31, 2, x_29);
+lean_ctor_set(x_12, 0, x_31);
+return x_12;
+}
+else
+{
+lean_object* x_32; lean_object* x_33; lean_object* x_34; lean_object* x_35; lean_object* x_36; lean_object* x_37; lean_object* x_38; lean_object* x_39; lean_object* x_40; lean_object* x_41; lean_object* x_42; lean_object* x_43; lean_object* x_44; lean_object* x_45; lean_object* x_46; lean_object* x_47; lean_object* x_48; lean_object* x_49; lean_object* x_50; lean_object* x_51; 
+x_32 = lean_ctor_get(x_12, 0);
+x_33 = lean_ctor_get(x_12, 1);
+lean_inc(x_33);
+lean_inc(x_32);
+lean_dec(x_12);
+x_34 = lean_ctor_get(x_2, 2);
+lean_inc(x_34);
+x_35 = lean_ctor_get(x_2, 1);
+lean_inc(x_35);
+lean_dec(x_2);
+x_36 = l_prover___aux__Src__Prover__Set______macroRules__prover__term___u2208____1___closed__12;
+x_37 = l_Lean_addMacroScope(x_35, x_36, x_34);
+x_38 = l_prover___aux__Src__Prover__Set______macroRules__prover__term___u2208____1___closed__11;
+x_39 = l_prover___aux__Src__Prover__Set______macroRules__prover__term___u2208____1___closed__15;
+x_40 = lean_alloc_ctor(3, 4, 0);
+lean_ctor_set(x_40, 0, x_32);
+lean_ctor_set(x_40, 1, x_38);
+lean_ctor_set(x_40, 2, x_37);
+lean_ctor_set(x_40, 3, x_39);
+x_41 = l_prover___aux__Src__Prover__Set______macroRules__prover__term___u2208____1___closed__18;
+x_42 = lean_array_push(x_41, x_9);
+x_43 = lean_array_push(x_42, x_11);
+x_44 = lean_box(2);
+x_45 = l_prover___aux__Src__Prover__Set______macroRules__prover__term___u2208____1___closed__17;
+x_46 = lean_alloc_ctor(1, 3, 0);
+lean_ctor_set(x_46, 0, x_44);
+lean_ctor_set(x_46, 1, x_45);
+lean_ctor_set(x_46, 2, x_43);
+x_47 = lean_array_push(x_41, x_40);
+x_48 = lean_array_push(x_47, x_46);
+x_49 = l_prover___aux__Src__Prover__Set______macroRules__prover__term___u2208____1___closed__8;
+x_50 = lean_alloc_ctor(1, 3, 0);
+lean_ctor_set(x_50, 0, x_44);
+lean_ctor_set(x_50, 1, x_49);
+lean_ctor_set(x_50, 2, x_48);
+x_51 = lean_alloc_ctor(0, 2, 0);
+lean_ctor_set(x_51, 0, x_50);
+lean_ctor_set(x_51, 1, x_33);
+return x_51;
+}
+}
+}
+}
+static lean_object* _init_l_prover___aux__Src__Prover__Set______unexpand__prover__mem__1___closed__1() {
+_start:
+{
+lean_object* x_1; 
+x_1 = lean_mk_string_from_bytes("ident", 5);
+return x_1;
+}
+}
+static lean_object* _init_l_prover___aux__Src__Prover__Set______unexpand__prover__mem__1___closed__2() {
+_start:
+{
+lean_object* x_1; lean_object* x_2; lean_object* x_3; 
+x_1 = lean_box(0);
+x_2 = l_prover___aux__Src__Prover__Set______unexpand__prover__mem__1___closed__1;
+x_3 = lean_name_mk_string(x_1, x_2);
+return x_3;
+}
+}
+static lean_object* _init_l_prover___aux__Src__Prover__Set______unexpand__prover__mem__1___closed__3() {
+_start:
+{
+lean_object* x_1; lean_object* x_2; 
+x_1 = lean_unsigned_to_nat(3u);
+x_2 = lean_mk_empty_array_with_capacity(x_1);
+return x_2;
+}
+}
+LEAN_EXPORT lean_object* l_prover___aux__Src__Prover__Set______unexpand__prover__mem__1(lean_object* x_1, lean_object* x_2, lean_object* x_3) {
+_start:
+{
+lean_object* x_4; uint8_t x_5; 
+x_4 = l_prover___aux__Src__Prover__Set______macroRules__prover__term___u2208____1___closed__8;
+lean_inc(x_1);
+x_5 = l_Lean_Syntax_isOfKind(x_1, x_4);
+if (x_5 == 0)
+{
+lean_object* x_6; lean_object* x_7; 
+lean_dec(x_1);
+x_6 = lean_box(0);
+x_7 = lean_alloc_ctor(1, 2, 0);
+lean_ctor_set(x_7, 0, x_6);
+lean_ctor_set(x_7, 1, x_3);
+return x_7;
+}
+else
+{
+lean_object* x_8; lean_object* x_9; lean_object* x_10; uint8_t x_11; 
+x_8 = lean_unsigned_to_nat(0u);
+x_9 = l_Lean_Syntax_getArg(x_1, x_8);
+x_10 = l_prover___aux__Src__Prover__Set______unexpand__prover__mem__1___closed__2;
+lean_inc(x_9);
+x_11 = l_Lean_Syntax_isOfKind(x_9, x_10);
+if (x_11 == 0)
+{
+lean_object* x_12; lean_object* x_13; 
+lean_dec(x_9);
+lean_dec(x_1);
+x_12 = lean_box(0);
+x_13 = lean_alloc_ctor(1, 2, 0);
+lean_ctor_set(x_13, 0, x_12);
+lean_ctor_set(x_13, 1, x_3);
+return x_13;
+}
+else
+{
+lean_object* x_14; lean_object* x_15; lean_object* x_16; lean_object* x_17; uint8_t x_18; 
+x_14 = lean_unsigned_to_nat(1u);
+x_15 = l_Lean_Syntax_getArg(x_1, x_14);
+lean_dec(x_1);
+x_16 = l_Lean_nullKind;
+x_17 = lean_unsigned_to_nat(2u);
+lean_inc(x_15);
+x_18 = l_Lean_Syntax_isNodeOf(x_15, x_16, x_17);
+if (x_18 == 0)
+{
+lean_object* x_19; lean_object* x_20; 
+lean_dec(x_15);
+lean_dec(x_9);
+x_19 = lean_box(0);
+x_20 = lean_alloc_ctor(1, 2, 0);
+lean_ctor_set(x_20, 0, x_19);
+lean_ctor_set(x_20, 1, x_3);
+return x_20;
+}
+else
+{
+lean_object* x_21; lean_object* x_22; lean_object* x_23; lean_object* x_24; uint8_t x_25; 
+x_21 = l_Lean_Syntax_getArg(x_15, x_8);
+x_22 = l_Lean_Syntax_getArg(x_15, x_14);
+lean_dec(x_15);
+x_23 = l_Lean_replaceRef(x_9, x_2);
+lean_dec(x_9);
+x_24 = l_Lean_MonadRef_mkInfoFromRefPos___at___aux__Init__Notation______unexpand__Function__comp__1___spec__1(x_23, x_3);
+x_25 = !lean_is_exclusive(x_24);
+if (x_25 == 0)
+{
+lean_object* x_26; lean_object* x_27; lean_object* x_28; lean_object* x_29; lean_object* x_30; lean_object* x_31; lean_object* x_32; lean_object* x_33; lean_object* x_34; lean_object* x_35; 
+x_26 = lean_ctor_get(x_24, 0);
+x_27 = l_prover_term___u2208_____closed__7;
+x_28 = lean_alloc_ctor(2, 2, 0);
+lean_ctor_set(x_28, 0, x_26);
+lean_ctor_set(x_28, 1, x_27);
+x_29 = l_prover___aux__Src__Prover__Set______unexpand__prover__mem__1___closed__3;
+x_30 = lean_array_push(x_29, x_21);
+x_31 = lean_array_push(x_30, x_28);
+x_32 = lean_array_push(x_31, x_22);
+x_33 = lean_box(2);
+x_34 = l_prover_term___u2208_____closed__4;
+x_35 = lean_alloc_ctor(1, 3, 0);
+lean_ctor_set(x_35, 0, x_33);
+lean_ctor_set(x_35, 1, x_34);
+lean_ctor_set(x_35, 2, x_32);
+lean_ctor_set(x_24, 0, x_35);
+return x_24;
+}
+else
+{
+lean_object* x_36; lean_object* x_37; lean_object* x_38; lean_object* x_39; lean_object* x_40; lean_object* x_41; lean_object* x_42; lean_object* x_43; lean_object* x_44; lean_object* x_45; lean_object* x_46; lean_object* x_47; 
+x_36 = lean_ctor_get(x_24, 0);
+x_37 = lean_ctor_get(x_24, 1);
+lean_inc(x_37);
+lean_inc(x_36);
+lean_dec(x_24);
+x_38 = l_prover_term___u2208_____closed__7;
+x_39 = lean_alloc_ctor(2, 2, 0);
+lean_ctor_set(x_39, 0, x_36);
+lean_ctor_set(x_39, 1, x_38);
+x_40 = l_prover___aux__Src__Prover__Set______unexpand__prover__mem__1___closed__3;
+x_41 = lean_array_push(x_40, x_21);
+x_42 = lean_array_push(x_41, x_39);
+x_43 = lean_array_push(x_42, x_22);
+x_44 = lean_box(2);
+x_45 = l_prover_term___u2208_____closed__4;
+x_46 = lean_alloc_ctor(1, 3, 0);
+lean_ctor_set(x_46, 0, x_44);
+lean_ctor_set(x_46, 1, x_45);
+lean_ctor_set(x_46, 2, x_43);
+x_47 = lean_alloc_ctor(0, 2, 0);
+lean_ctor_set(x_47, 0, x_46);
+lean_ctor_set(x_47, 1, x_37);
+return x_47;
+}
+}
+}
+}
+}
+}
+LEAN_EXPORT lean_object* l_prover___aux__Src__Prover__Set______unexpand__prover__mem__1___boxed(lean_object* x_1, lean_object* x_2, lean_object* x_3) {
+_start:
+{
+lean_object* x_4; 
+x_4 = l_prover___aux__Src__Prover__Set______unexpand__prover__mem__1(x_1, x_2, x_3);
+lean_dec(x_2);
+return x_4;
+}
+}
+static lean_object* _init_l_prover_term___u2209_____closed__1() {
+_start:
+{
+lean_object* x_1; 
+x_1 = lean_mk_string_from_bytes("term_∉_", 9);
+return x_1;
+}
+}
+static lean_object* _init_l_prover_term___u2209_____closed__2() {
+_start:
+{
+lean_object* x_1; lean_object* x_2; lean_object* x_3; 
+x_1 = l_prover_term___u2208_____closed__2;
+x_2 = l_prover_term___u2209_____closed__1;
+x_3 = lean_name_mk_string(x_1, x_2);
+return x_3;
+}
+}
+static lean_object* _init_l_prover_term___u2209_____closed__3() {
+_start:
+{
+lean_object* x_1; 
+x_1 = lean_mk_string_from_bytes(" ∉ ", 5);
+return x_1;
+}
+}
+static lean_object* _init_l_prover_term___u2209_____closed__4() {
+_start:
+{
+lean_object* x_1; lean_object* x_2; 
+x_1 = l_prover_term___u2209_____closed__3;
+x_2 = lean_alloc_ctor(5, 1, 0);
+lean_ctor_set(x_2, 0, x_1);
+return x_2;
+}
+}
+static lean_object* _init_l_prover_term___u2209_____closed__5() {
+_start:
+{
+lean_object* x_1; lean_object* x_2; lean_object* x_3; lean_object* x_4; 
+x_1 = l_prover_term___u2208_____closed__6;
+x_2 = l_prover_term___u2209_____closed__4;
+x_3 = l_prover_term___u2208_____closed__11;
+x_4 = lean_alloc_ctor(2, 3, 0);
+lean_ctor_set(x_4, 0, x_1);
+lean_ctor_set(x_4, 1, x_2);
+lean_ctor_set(x_4, 2, x_3);
+return x_4;
+}
+}
+static lean_object* _init_l_prover_term___u2209_____closed__6() {
+_start:
+{
+lean_object* x_1; lean_object* x_2; lean_object* x_3; lean_object* x_4; lean_object* x_5; 
+x_1 = l_prover_term___u2209_____closed__2;
+x_2 = lean_unsigned_to_nat(50u);
+x_3 = lean_unsigned_to_nat(51u);
+x_4 = l_prover_term___u2209_____closed__5;
+x_5 = lean_alloc_ctor(4, 4, 0);
+lean_ctor_set(x_5, 0, x_1);
+lean_ctor_set(x_5, 1, x_2);
+lean_ctor_set(x_5, 2, x_3);
+lean_ctor_set(x_5, 3, x_4);
+return x_5;
+}
+}
+static lean_object* _init_l_prover_term___u2209__() {
+_start:
+{
+lean_object* x_1; 
+x_1 = l_prover_term___u2209_____closed__6;
+return x_1;
+}
+}
+static lean_object* _init_l_prover___aux__Src__Prover__Set______macroRules__prover__term___u2209____1___closed__1() {
+_start:
+{
+lean_object* x_1; 
+x_1 = lean_mk_string_from_bytes("not_mem", 7);
+return x_1;
+}
+}
+static lean_object* _init_l_prover___aux__Src__Prover__Set______macroRules__prover__term___u2209____1___closed__2() {
+_start:
+{
+lean_object* x_1; lean_object* x_2; 
+x_1 = l_prover___aux__Src__Prover__Set______macroRules__prover__term___u2209____1___closed__1;
+x_2 = lean_string_utf8_byte_size(x_1);
+return x_2;
+}
+}
+static lean_object* _init_l_prover___aux__Src__Prover__Set______macroRules__prover__term___u2209____1___closed__3() {
+_start:
+{
+lean_object* x_1; lean_object* x_2; lean_object* x_3; lean_object* x_4; 
+x_1 = l_prover___aux__Src__Prover__Set______macroRules__prover__term___u2209____1___closed__1;
+x_2 = lean_unsigned_to_nat(0u);
+x_3 = l_prover___aux__Src__Prover__Set______macroRules__prover__term___u2209____1___closed__2;
+x_4 = lean_alloc_ctor(0, 3, 0);
+lean_ctor_set(x_4, 0, x_1);
+lean_ctor_set(x_4, 1, x_2);
+lean_ctor_set(x_4, 2, x_3);
+return x_4;
+}
+}
+static lean_object* _init_l_prover___aux__Src__Prover__Set______macroRules__prover__term___u2209____1___closed__4() {
+_start:
+{
+lean_object* x_1; lean_object* x_2; lean_object* x_3; 
+x_1 = lean_box(0);
+x_2 = l_prover___aux__Src__Prover__Set______macroRules__prover__term___u2209____1___closed__1;
+x_3 = lean_name_mk_string(x_1, x_2);
+return x_3;
+}
+}
+static lean_object* _init_l_prover___aux__Src__Prover__Set______macroRules__prover__term___u2209____1___closed__5() {
+_start:
+{
+lean_object* x_1; lean_object* x_2; lean_object* x_3; 
+x_1 = l_prover_term___u2208_____closed__2;
+x_2 = l_prover___aux__Src__Prover__Set______macroRules__prover__term___u2209____1___closed__1;
+x_3 = lean_name_mk_string(x_1, x_2);
+return x_3;
+}
+}
+static lean_object* _init_l_prover___aux__Src__Prover__Set______macroRules__prover__term___u2209____1___closed__6() {
+_start:
+{
+lean_object* x_1; lean_object* x_2; lean_object* x_3; 
+x_1 = lean_box(0);
+x_2 = l_prover___aux__Src__Prover__Set______macroRules__prover__term___u2209____1___closed__5;
+x_3 = lean_alloc_ctor(0, 2, 0);
+lean_ctor_set(x_3, 0, x_2);
+lean_ctor_set(x_3, 1, x_1);
+return x_3;
+}
+}
+static lean_object* _init_l_prover___aux__Src__Prover__Set______macroRules__prover__term___u2209____1___closed__7() {
+_start:
+{
+lean_object* x_1; lean_object* x_2; lean_object* x_3; 
+x_1 = lean_box(0);
+x_2 = l_prover___aux__Src__Prover__Set______macroRules__prover__term___u2209____1___closed__6;
+x_3 = lean_alloc_ctor(1, 2, 0);
+lean_ctor_set(x_3, 0, x_2);
+lean_ctor_set(x_3, 1, x_1);
+return x_3;
+}
+}
+LEAN_EXPORT lean_object* l_prover___aux__Src__Prover__Set______macroRules__prover__term___u2209____1(lean_object* x_1, lean_object* x_2, lean_object* x_3) {
+_start:
+{
+lean_object* x_4; uint8_t x_5; 
+x_4 = l_prover_term___u2209_____closed__2;
+lean_inc(x_1);
+x_5 = l_Lean_Syntax_isOfKind(x_1, x_4);
+if (x_5 == 0)
+{
+lean_object* x_6; lean_object* x_7; 
+lean_dec(x_2);
+lean_dec(x_1);
+x_6 = lean_box(1);
+x_7 = lean_alloc_ctor(1, 2, 0);
+lean_ctor_set(x_7, 0, x_6);
+lean_ctor_set(x_7, 1, x_3);
+return x_7;
+}
+else
+{
+lean_object* x_8; lean_object* x_9; lean_object* x_10; lean_object* x_11; lean_object* x_12; uint8_t x_13; 
+x_8 = lean_unsigned_to_nat(0u);
+x_9 = l_Lean_Syntax_getArg(x_1, x_8);
+x_10 = lean_unsigned_to_nat(2u);
+x_11 = l_Lean_Syntax_getArg(x_1, x_10);
+lean_dec(x_1);
+lean_inc(x_2);
+x_12 = l_Lean_MonadRef_mkInfoFromRefPos___at___aux__Init__Notation______macroRules__precMax__1___spec__1(x_2, x_3);
+x_13 = !lean_is_exclusive(x_12);
+if (x_13 == 0)
+{
+lean_object* x_14; lean_object* x_15; lean_object* x_16; lean_object* x_17; lean_object* x_18; lean_object* x_19; lean_object* x_20; lean_object* x_21; lean_object* x_22; lean_object* x_23; lean_object* x_24; lean_object* x_25; lean_object* x_26; lean_object* x_27; lean_object* x_28; lean_object* x_29; lean_object* x_30; lean_object* x_31; 
+x_14 = lean_ctor_get(x_12, 0);
+x_15 = lean_ctor_get(x_2, 2);
+lean_inc(x_15);
+x_16 = lean_ctor_get(x_2, 1);
+lean_inc(x_16);
+lean_dec(x_2);
+x_17 = l_prover___aux__Src__Prover__Set______macroRules__prover__term___u2209____1___closed__4;
+x_18 = l_Lean_addMacroScope(x_16, x_17, x_15);
+x_19 = l_prover___aux__Src__Prover__Set______macroRules__prover__term___u2209____1___closed__3;
+x_20 = l_prover___aux__Src__Prover__Set______macroRules__prover__term___u2209____1___closed__7;
+x_21 = lean_alloc_ctor(3, 4, 0);
+lean_ctor_set(x_21, 0, x_14);
+lean_ctor_set(x_21, 1, x_19);
+lean_ctor_set(x_21, 2, x_18);
+lean_ctor_set(x_21, 3, x_20);
+x_22 = l_prover___aux__Src__Prover__Set______macroRules__prover__term___u2208____1___closed__18;
+x_23 = lean_array_push(x_22, x_9);
+x_24 = lean_array_push(x_23, x_11);
+x_25 = lean_box(2);
+x_26 = l_prover___aux__Src__Prover__Set______macroRules__prover__term___u2208____1___closed__17;
+x_27 = lean_alloc_ctor(1, 3, 0);
+lean_ctor_set(x_27, 0, x_25);
+lean_ctor_set(x_27, 1, x_26);
+lean_ctor_set(x_27, 2, x_24);
+x_28 = lean_array_push(x_22, x_21);
+x_29 = lean_array_push(x_28, x_27);
+x_30 = l_prover___aux__Src__Prover__Set______macroRules__prover__term___u2208____1___closed__8;
+x_31 = lean_alloc_ctor(1, 3, 0);
+lean_ctor_set(x_31, 0, x_25);
+lean_ctor_set(x_31, 1, x_30);
+lean_ctor_set(x_31, 2, x_29);
+lean_ctor_set(x_12, 0, x_31);
+return x_12;
+}
+else
+{
+lean_object* x_32; lean_object* x_33; lean_object* x_34; lean_object* x_35; lean_object* x_36; lean_object* x_37; lean_object* x_38; lean_object* x_39; lean_object* x_40; lean_object* x_41; lean_object* x_42; lean_object* x_43; lean_object* x_44; lean_object* x_45; lean_object* x_46; lean_object* x_47; lean_object* x_48; lean_object* x_49; lean_object* x_50; lean_object* x_51; 
+x_32 = lean_ctor_get(x_12, 0);
+x_33 = lean_ctor_get(x_12, 1);
+lean_inc(x_33);
+lean_inc(x_32);
+lean_dec(x_12);
+x_34 = lean_ctor_get(x_2, 2);
+lean_inc(x_34);
+x_35 = lean_ctor_get(x_2, 1);
+lean_inc(x_35);
+lean_dec(x_2);
+x_36 = l_prover___aux__Src__Prover__Set______macroRules__prover__term___u2209____1___closed__4;
+x_37 = l_Lean_addMacroScope(x_35, x_36, x_34);
+x_38 = l_prover___aux__Src__Prover__Set______macroRules__prover__term___u2209____1___closed__3;
+x_39 = l_prover___aux__Src__Prover__Set______macroRules__prover__term___u2209____1___closed__7;
+x_40 = lean_alloc_ctor(3, 4, 0);
+lean_ctor_set(x_40, 0, x_32);
+lean_ctor_set(x_40, 1, x_38);
+lean_ctor_set(x_40, 2, x_37);
+lean_ctor_set(x_40, 3, x_39);
+x_41 = l_prover___aux__Src__Prover__Set______macroRules__prover__term___u2208____1___closed__18;
+x_42 = lean_array_push(x_41, x_9);
+x_43 = lean_array_push(x_42, x_11);
+x_44 = lean_box(2);
+x_45 = l_prover___aux__Src__Prover__Set______macroRules__prover__term___u2208____1___closed__17;
+x_46 = lean_alloc_ctor(1, 3, 0);
+lean_ctor_set(x_46, 0, x_44);
+lean_ctor_set(x_46, 1, x_45);
+lean_ctor_set(x_46, 2, x_43);
+x_47 = lean_array_push(x_41, x_40);
+x_48 = lean_array_push(x_47, x_46);
+x_49 = l_prover___aux__Src__Prover__Set______macroRules__prover__term___u2208____1___closed__8;
+x_50 = lean_alloc_ctor(1, 3, 0);
+lean_ctor_set(x_50, 0, x_44);
+lean_ctor_set(x_50, 1, x_49);
+lean_ctor_set(x_50, 2, x_48);
+x_51 = lean_alloc_ctor(0, 2, 0);
+lean_ctor_set(x_51, 0, x_50);
+lean_ctor_set(x_51, 1, x_33);
+return x_51;
+}
+}
+}
+}
+LEAN_EXPORT lean_object* l_prover___aux__Src__Prover__Set______unexpand__prover__not__mem__1(lean_object* x_1, lean_object* x_2, lean_object* x_3) {
+_start:
+{
+lean_object* x_4; uint8_t x_5; 
+x_4 = l_prover___aux__Src__Prover__Set______macroRules__prover__term___u2208____1___closed__8;
+lean_inc(x_1);
+x_5 = l_Lean_Syntax_isOfKind(x_1, x_4);
+if (x_5 == 0)
+{
+lean_object* x_6; lean_object* x_7; 
+lean_dec(x_1);
+x_6 = lean_box(0);
+x_7 = lean_alloc_ctor(1, 2, 0);
+lean_ctor_set(x_7, 0, x_6);
+lean_ctor_set(x_7, 1, x_3);
+return x_7;
+}
+else
+{
+lean_object* x_8; lean_object* x_9; lean_object* x_10; uint8_t x_11; 
+x_8 = lean_unsigned_to_nat(0u);
+x_9 = l_Lean_Syntax_getArg(x_1, x_8);
+x_10 = l_prover___aux__Src__Prover__Set______unexpand__prover__mem__1___closed__2;
+lean_inc(x_9);
+x_11 = l_Lean_Syntax_isOfKind(x_9, x_10);
+if (x_11 == 0)
+{
+lean_object* x_12; lean_object* x_13; 
+lean_dec(x_9);
+lean_dec(x_1);
+x_12 = lean_box(0);
+x_13 = lean_alloc_ctor(1, 2, 0);
+lean_ctor_set(x_13, 0, x_12);
+lean_ctor_set(x_13, 1, x_3);
+return x_13;
+}
+else
+{
+lean_object* x_14; lean_object* x_15; lean_object* x_16; lean_object* x_17; uint8_t x_18; 
+x_14 = lean_unsigned_to_nat(1u);
+x_15 = l_Lean_Syntax_getArg(x_1, x_14);
+lean_dec(x_1);
+x_16 = l_Lean_nullKind;
+x_17 = lean_unsigned_to_nat(2u);
+lean_inc(x_15);
+x_18 = l_Lean_Syntax_isNodeOf(x_15, x_16, x_17);
+if (x_18 == 0)
+{
+lean_object* x_19; lean_object* x_20; 
+lean_dec(x_15);
+lean_dec(x_9);
+x_19 = lean_box(0);
+x_20 = lean_alloc_ctor(1, 2, 0);
+lean_ctor_set(x_20, 0, x_19);
+lean_ctor_set(x_20, 1, x_3);
+return x_20;
+}
+else
+{
+lean_object* x_21; lean_object* x_22; lean_object* x_23; lean_object* x_24; uint8_t x_25; 
+x_21 = l_Lean_Syntax_getArg(x_15, x_8);
+x_22 = l_Lean_Syntax_getArg(x_15, x_14);
+lean_dec(x_15);
+x_23 = l_Lean_replaceRef(x_9, x_2);
+lean_dec(x_9);
+x_24 = l_Lean_MonadRef_mkInfoFromRefPos___at___aux__Init__Notation______unexpand__Function__comp__1___spec__1(x_23, x_3);
+x_25 = !lean_is_exclusive(x_24);
+if (x_25 == 0)
+{
+lean_object* x_26; lean_object* x_27; lean_object* x_28; lean_object* x_29; lean_object* x_30; lean_object* x_31; lean_object* x_32; lean_object* x_33; lean_object* x_34; lean_object* x_35; 
+x_26 = lean_ctor_get(x_24, 0);
+x_27 = l_prover_term___u2209_____closed__3;
+x_28 = lean_alloc_ctor(2, 2, 0);
+lean_ctor_set(x_28, 0, x_26);
+lean_ctor_set(x_28, 1, x_27);
+x_29 = l_prover___aux__Src__Prover__Set______unexpand__prover__mem__1___closed__3;
+x_30 = lean_array_push(x_29, x_21);
+x_31 = lean_array_push(x_30, x_28);
+x_32 = lean_array_push(x_31, x_22);
+x_33 = lean_box(2);
+x_34 = l_prover_term___u2209_____closed__2;
+x_35 = lean_alloc_ctor(1, 3, 0);
+lean_ctor_set(x_35, 0, x_33);
+lean_ctor_set(x_35, 1, x_34);
+lean_ctor_set(x_35, 2, x_32);
+lean_ctor_set(x_24, 0, x_35);
+return x_24;
+}
+else
+{
+lean_object* x_36; lean_object* x_37; lean_object* x_38; lean_object* x_39; lean_object* x_40; lean_object* x_41; lean_object* x_42; lean_object* x_43; lean_object* x_44; lean_object* x_45; lean_object* x_46; lean_object* x_47; 
+x_36 = lean_ctor_get(x_24, 0);
+x_37 = lean_ctor_get(x_24, 1);
+lean_inc(x_37);
+lean_inc(x_36);
+lean_dec(x_24);
+x_38 = l_prover_term___u2209_____closed__3;
+x_39 = lean_alloc_ctor(2, 2, 0);
+lean_ctor_set(x_39, 0, x_36);
+lean_ctor_set(x_39, 1, x_38);
+x_40 = l_prover___aux__Src__Prover__Set______unexpand__prover__mem__1___closed__3;
+x_41 = lean_array_push(x_40, x_21);
+x_42 = lean_array_push(x_41, x_39);
+x_43 = lean_array_push(x_42, x_22);
+x_44 = lean_box(2);
+x_45 = l_prover_term___u2209_____closed__2;
+x_46 = lean_alloc_ctor(1, 3, 0);
+lean_ctor_set(x_46, 0, x_44);
+lean_ctor_set(x_46, 1, x_45);
+lean_ctor_set(x_46, 2, x_43);
+x_47 = lean_alloc_ctor(0, 2, 0);
+lean_ctor_set(x_47, 0, x_46);
+lean_ctor_set(x_47, 1, x_37);
+return x_47;
+}
+}
+}
+}
+}
+}
+LEAN_EXPORT lean_object* l_prover___aux__Src__Prover__Set______unexpand__prover__not__mem__1___boxed(lean_object* x_1, lean_object* x_2, lean_object* x_3) {
+_start:
+{
+lean_object* x_4; 
+x_4 = l_prover___aux__Src__Prover__Set______unexpand__prover__not__mem__1(x_1, x_2, x_3);
+lean_dec(x_2);
+return x_4;
+}
+}
+static lean_object* _init_l_prover_term___u2286_____closed__1() {
+_start:
+{
+lean_object* x_1; 
+x_1 = lean_mk_string_from_bytes("term_⊆_", 9);
+return x_1;
+}
+}
+static lean_object* _init_l_prover_term___u2286_____closed__2() {
+_start:
+{
+lean_object* x_1; lean_object* x_2; lean_object* x_3; 
+x_1 = l_prover_term___u2208_____closed__2;
+x_2 = l_prover_term___u2286_____closed__1;
+x_3 = lean_name_mk_string(x_1, x_2);
+return x_3;
+}
+}
+static lean_object* _init_l_prover_term___u2286_____closed__3() {
+_start:
+{
+lean_object* x_1; 
+x_1 = lean_mk_string_from_bytes(" ⊆ ", 5);
+return x_1;
+}
+}
+static lean_object* _init_l_prover_term___u2286_____closed__4() {
+_start:
+{
+lean_object* x_1; lean_object* x_2; 
+x_1 = l_prover_term___u2286_____closed__3;
+x_2 = lean_alloc_ctor(5, 1, 0);
+lean_ctor_set(x_2, 0, x_1);
+return x_2;
+}
+}
+static lean_object* _init_l_prover_term___u2286_____closed__5() {
+_start:
+{
+lean_object* x_1; lean_object* x_2; lean_object* x_3; lean_object* x_4; 
+x_1 = l_prover_term___u2208_____closed__6;
+x_2 = l_prover_term___u2286_____closed__4;
+x_3 = l_prover_term___u2208_____closed__11;
+x_4 = lean_alloc_ctor(2, 3, 0);
+lean_ctor_set(x_4, 0, x_1);
+lean_ctor_set(x_4, 1, x_2);
+lean_ctor_set(x_4, 2, x_3);
+return x_4;
+}
+}
+static lean_object* _init_l_prover_term___u2286_____closed__6() {
+_start:
+{
+lean_object* x_1; lean_object* x_2; lean_object* x_3; lean_object* x_4; lean_object* x_5; 
+x_1 = l_prover_term___u2286_____closed__2;
+x_2 = lean_unsigned_to_nat(50u);
+x_3 = lean_unsigned_to_nat(51u);
+x_4 = l_prover_term___u2286_____closed__5;
+x_5 = lean_alloc_ctor(4, 4, 0);
+lean_ctor_set(x_5, 0, x_1);
+lean_ctor_set(x_5, 1, x_2);
+lean_ctor_set(x_5, 2, x_3);
+lean_ctor_set(x_5, 3, x_4);
+return x_5;
+}
+}
+static lean_object* _init_l_prover_term___u2286__() {
+_start:
+{
+lean_object* x_1; 
+x_1 = l_prover_term___u2286_____closed__6;
+return x_1;
+}
+}
+static lean_object* _init_l_prover___aux__Src__Prover__Set______macroRules__prover__term___u2286____1___closed__1() {
+_start:
+{
+lean_object* x_1; 
+x_1 = lean_mk_string_from_bytes("subset", 6);
+return x_1;
+}
+}
+static lean_object* _init_l_prover___aux__Src__Prover__Set______macroRules__prover__term___u2286____1___closed__2() {
+_start:
+{
+lean_object* x_1; lean_object* x_2; 
+x_1 = l_prover___aux__Src__Prover__Set______macroRules__prover__term___u2286____1___closed__1;
+x_2 = lean_string_utf8_byte_size(x_1);
+return x_2;
+}
+}
+static lean_object* _init_l_prover___aux__Src__Prover__Set______macroRules__prover__term___u2286____1___closed__3() {
+_start:
+{
+lean_object* x_1; lean_object* x_2; lean_object* x_3; lean_object* x_4; 
+x_1 = l_prover___aux__Src__Prover__Set______macroRules__prover__term___u2286____1___closed__1;
+x_2 = lean_unsigned_to_nat(0u);
+x_3 = l_prover___aux__Src__Prover__Set______macroRules__prover__term___u2286____1___closed__2;
+x_4 = lean_alloc_ctor(0, 3, 0);
+lean_ctor_set(x_4, 0, x_1);
+lean_ctor_set(x_4, 1, x_2);
+lean_ctor_set(x_4, 2, x_3);
+return x_4;
+}
+}
+static lean_object* _init_l_prover___aux__Src__Prover__Set______macroRules__prover__term___u2286____1___closed__4() {
+_start:
+{
+lean_object* x_1; lean_object* x_2; lean_object* x_3; 
+x_1 = lean_box(0);
+x_2 = l_prover___aux__Src__Prover__Set______macroRules__prover__term___u2286____1___closed__1;
+x_3 = lean_name_mk_string(x_1, x_2);
+return x_3;
+}
+}
+static lean_object* _init_l_prover___aux__Src__Prover__Set______macroRules__prover__term___u2286____1___closed__5() {
+_start:
+{
+lean_object* x_1; lean_object* x_2; lean_object* x_3; 
+x_1 = l_prover_term___u2208_____closed__2;
+x_2 = l_prover___aux__Src__Prover__Set______macroRules__prover__term___u2286____1___closed__1;
+x_3 = lean_name_mk_string(x_1, x_2);
+return x_3;
+}
+}
+static lean_object* _init_l_prover___aux__Src__Prover__Set______macroRules__prover__term___u2286____1___closed__6() {
+_start:
+{
+lean_object* x_1; lean_object* x_2; lean_object* x_3; 
+x_1 = lean_box(0);
+x_2 = l_prover___aux__Src__Prover__Set______macroRules__prover__term___u2286____1___closed__5;
+x_3 = lean_alloc_ctor(0, 2, 0);
+lean_ctor_set(x_3, 0, x_2);
+lean_ctor_set(x_3, 1, x_1);
+return x_3;
+}
+}
+static lean_object* _init_l_prover___aux__Src__Prover__Set______macroRules__prover__term___u2286____1___closed__7() {
+_start:
+{
+lean_object* x_1; lean_object* x_2; lean_object* x_3; 
+x_1 = lean_box(0);
+x_2 = l_prover___aux__Src__Prover__Set______macroRules__prover__term___u2286____1___closed__6;
+x_3 = lean_alloc_ctor(1, 2, 0);
+lean_ctor_set(x_3, 0, x_2);
+lean_ctor_set(x_3, 1, x_1);
+return x_3;
+}
+}
+LEAN_EXPORT lean_object* l_prover___aux__Src__Prover__Set______macroRules__prover__term___u2286____1(lean_object* x_1, lean_object* x_2, lean_object* x_3) {
+_start:
+{
+lean_object* x_4; uint8_t x_5; 
+x_4 = l_prover_term___u2286_____closed__2;
+lean_inc(x_1);
+x_5 = l_Lean_Syntax_isOfKind(x_1, x_4);
+if (x_5 == 0)
+{
+lean_object* x_6; lean_object* x_7; 
+lean_dec(x_2);
+lean_dec(x_1);
+x_6 = lean_box(1);
+x_7 = lean_alloc_ctor(1, 2, 0);
+lean_ctor_set(x_7, 0, x_6);
+lean_ctor_set(x_7, 1, x_3);
+return x_7;
+}
+else
+{
+lean_object* x_8; lean_object* x_9; lean_object* x_10; lean_object* x_11; lean_object* x_12; uint8_t x_13; 
+x_8 = lean_unsigned_to_nat(0u);
+x_9 = l_Lean_Syntax_getArg(x_1, x_8);
+x_10 = lean_unsigned_to_nat(2u);
+x_11 = l_Lean_Syntax_getArg(x_1, x_10);
+lean_dec(x_1);
+lean_inc(x_2);
+x_12 = l_Lean_MonadRef_mkInfoFromRefPos___at___aux__Init__Notation______macroRules__precMax__1___spec__1(x_2, x_3);
+x_13 = !lean_is_exclusive(x_12);
+if (x_13 == 0)
+{
+lean_object* x_14; lean_object* x_15; lean_object* x_16; lean_object* x_17; lean_object* x_18; lean_object* x_19; lean_object* x_20; lean_object* x_21; lean_object* x_22; lean_object* x_23; lean_object* x_24; lean_object* x_25; lean_object* x_26; lean_object* x_27; lean_object* x_28; lean_object* x_29; lean_object* x_30; lean_object* x_31; 
+x_14 = lean_ctor_get(x_12, 0);
+x_15 = lean_ctor_get(x_2, 2);
+lean_inc(x_15);
+x_16 = lean_ctor_get(x_2, 1);
+lean_inc(x_16);
+lean_dec(x_2);
+x_17 = l_prover___aux__Src__Prover__Set______macroRules__prover__term___u2286____1___closed__4;
+x_18 = l_Lean_addMacroScope(x_16, x_17, x_15);
+x_19 = l_prover___aux__Src__Prover__Set______macroRules__prover__term___u2286____1___closed__3;
+x_20 = l_prover___aux__Src__Prover__Set______macroRules__prover__term___u2286____1___closed__7;
+x_21 = lean_alloc_ctor(3, 4, 0);
+lean_ctor_set(x_21, 0, x_14);
+lean_ctor_set(x_21, 1, x_19);
+lean_ctor_set(x_21, 2, x_18);
+lean_ctor_set(x_21, 3, x_20);
+x_22 = l_prover___aux__Src__Prover__Set______macroRules__prover__term___u2208____1___closed__18;
+x_23 = lean_array_push(x_22, x_9);
+x_24 = lean_array_push(x_23, x_11);
+x_25 = lean_box(2);
+x_26 = l_prover___aux__Src__Prover__Set______macroRules__prover__term___u2208____1___closed__17;
+x_27 = lean_alloc_ctor(1, 3, 0);
+lean_ctor_set(x_27, 0, x_25);
+lean_ctor_set(x_27, 1, x_26);
+lean_ctor_set(x_27, 2, x_24);
+x_28 = lean_array_push(x_22, x_21);
+x_29 = lean_array_push(x_28, x_27);
+x_30 = l_prover___aux__Src__Prover__Set______macroRules__prover__term___u2208____1___closed__8;
+x_31 = lean_alloc_ctor(1, 3, 0);
+lean_ctor_set(x_31, 0, x_25);
+lean_ctor_set(x_31, 1, x_30);
+lean_ctor_set(x_31, 2, x_29);
+lean_ctor_set(x_12, 0, x_31);
+return x_12;
+}
+else
+{
+lean_object* x_32; lean_object* x_33; lean_object* x_34; lean_object* x_35; lean_object* x_36; lean_object* x_37; lean_object* x_38; lean_object* x_39; lean_object* x_40; lean_object* x_41; lean_object* x_42; lean_object* x_43; lean_object* x_44; lean_object* x_45; lean_object* x_46; lean_object* x_47; lean_object* x_48; lean_object* x_49; lean_object* x_50; lean_object* x_51; 
+x_32 = lean_ctor_get(x_12, 0);
+x_33 = lean_ctor_get(x_12, 1);
+lean_inc(x_33);
+lean_inc(x_32);
+lean_dec(x_12);
+x_34 = lean_ctor_get(x_2, 2);
+lean_inc(x_34);
+x_35 = lean_ctor_get(x_2, 1);
+lean_inc(x_35);
+lean_dec(x_2);
+x_36 = l_prover___aux__Src__Prover__Set______macroRules__prover__term___u2286____1___closed__4;
+x_37 = l_Lean_addMacroScope(x_35, x_36, x_34);
+x_38 = l_prover___aux__Src__Prover__Set______macroRules__prover__term___u2286____1___closed__3;
+x_39 = l_prover___aux__Src__Prover__Set______macroRules__prover__term___u2286____1___closed__7;
+x_40 = lean_alloc_ctor(3, 4, 0);
+lean_ctor_set(x_40, 0, x_32);
+lean_ctor_set(x_40, 1, x_38);
+lean_ctor_set(x_40, 2, x_37);
+lean_ctor_set(x_40, 3, x_39);
+x_41 = l_prover___aux__Src__Prover__Set______macroRules__prover__term___u2208____1___closed__18;
+x_42 = lean_array_push(x_41, x_9);
+x_43 = lean_array_push(x_42, x_11);
+x_44 = lean_box(2);
+x_45 = l_prover___aux__Src__Prover__Set______macroRules__prover__term___u2208____1___closed__17;
+x_46 = lean_alloc_ctor(1, 3, 0);
+lean_ctor_set(x_46, 0, x_44);
+lean_ctor_set(x_46, 1, x_45);
+lean_ctor_set(x_46, 2, x_43);
+x_47 = lean_array_push(x_41, x_40);
+x_48 = lean_array_push(x_47, x_46);
+x_49 = l_prover___aux__Src__Prover__Set______macroRules__prover__term___u2208____1___closed__8;
+x_50 = lean_alloc_ctor(1, 3, 0);
+lean_ctor_set(x_50, 0, x_44);
+lean_ctor_set(x_50, 1, x_49);
+lean_ctor_set(x_50, 2, x_48);
+x_51 = lean_alloc_ctor(0, 2, 0);
+lean_ctor_set(x_51, 0, x_50);
+lean_ctor_set(x_51, 1, x_33);
+return x_51;
+}
+}
+}
+}
+LEAN_EXPORT lean_object* l_prover___aux__Src__Prover__Set______unexpand__prover__subset__1(lean_object* x_1, lean_object* x_2, lean_object* x_3) {
+_start:
+{
+lean_object* x_4; uint8_t x_5; 
+x_4 = l_prover___aux__Src__Prover__Set______macroRules__prover__term___u2208____1___closed__8;
+lean_inc(x_1);
+x_5 = l_Lean_Syntax_isOfKind(x_1, x_4);
+if (x_5 == 0)
+{
+lean_object* x_6; lean_object* x_7; 
+lean_dec(x_1);
+x_6 = lean_box(0);
+x_7 = lean_alloc_ctor(1, 2, 0);
+lean_ctor_set(x_7, 0, x_6);
+lean_ctor_set(x_7, 1, x_3);
+return x_7;
+}
+else
+{
+lean_object* x_8; lean_object* x_9; lean_object* x_10; uint8_t x_11; 
+x_8 = lean_unsigned_to_nat(0u);
+x_9 = l_Lean_Syntax_getArg(x_1, x_8);
+x_10 = l_prover___aux__Src__Prover__Set______unexpand__prover__mem__1___closed__2;
+lean_inc(x_9);
+x_11 = l_Lean_Syntax_isOfKind(x_9, x_10);
+if (x_11 == 0)
+{
+lean_object* x_12; lean_object* x_13; 
+lean_dec(x_9);
+lean_dec(x_1);
+x_12 = lean_box(0);
+x_13 = lean_alloc_ctor(1, 2, 0);
+lean_ctor_set(x_13, 0, x_12);
+lean_ctor_set(x_13, 1, x_3);
+return x_13;
+}
+else
+{
+lean_object* x_14; lean_object* x_15; lean_object* x_16; lean_object* x_17; uint8_t x_18; 
+x_14 = lean_unsigned_to_nat(1u);
+x_15 = l_Lean_Syntax_getArg(x_1, x_14);
+lean_dec(x_1);
+x_16 = l_Lean_nullKind;
+x_17 = lean_unsigned_to_nat(2u);
+lean_inc(x_15);
+x_18 = l_Lean_Syntax_isNodeOf(x_15, x_16, x_17);
+if (x_18 == 0)
+{
+lean_object* x_19; lean_object* x_20; 
+lean_dec(x_15);
+lean_dec(x_9);
+x_19 = lean_box(0);
+x_20 = lean_alloc_ctor(1, 2, 0);
+lean_ctor_set(x_20, 0, x_19);
+lean_ctor_set(x_20, 1, x_3);
+return x_20;
+}
+else
+{
+lean_object* x_21; lean_object* x_22; lean_object* x_23; lean_object* x_24; uint8_t x_25; 
+x_21 = l_Lean_Syntax_getArg(x_15, x_8);
+x_22 = l_Lean_Syntax_getArg(x_15, x_14);
+lean_dec(x_15);
+x_23 = l_Lean_replaceRef(x_9, x_2);
+lean_dec(x_9);
+x_24 = l_Lean_MonadRef_mkInfoFromRefPos___at___aux__Init__Notation______unexpand__Function__comp__1___spec__1(x_23, x_3);
+x_25 = !lean_is_exclusive(x_24);
+if (x_25 == 0)
+{
+lean_object* x_26; lean_object* x_27; lean_object* x_28; lean_object* x_29; lean_object* x_30; lean_object* x_31; lean_object* x_32; lean_object* x_33; lean_object* x_34; lean_object* x_35; 
+x_26 = lean_ctor_get(x_24, 0);
+x_27 = l_prover_term___u2286_____closed__3;
+x_28 = lean_alloc_ctor(2, 2, 0);
+lean_ctor_set(x_28, 0, x_26);
+lean_ctor_set(x_28, 1, x_27);
+x_29 = l_prover___aux__Src__Prover__Set______unexpand__prover__mem__1___closed__3;
+x_30 = lean_array_push(x_29, x_21);
+x_31 = lean_array_push(x_30, x_28);
+x_32 = lean_array_push(x_31, x_22);
+x_33 = lean_box(2);
+x_34 = l_prover_term___u2286_____closed__2;
+x_35 = lean_alloc_ctor(1, 3, 0);
+lean_ctor_set(x_35, 0, x_33);
+lean_ctor_set(x_35, 1, x_34);
+lean_ctor_set(x_35, 2, x_32);
+lean_ctor_set(x_24, 0, x_35);
+return x_24;
+}
+else
+{
+lean_object* x_36; lean_object* x_37; lean_object* x_38; lean_object* x_39; lean_object* x_40; lean_object* x_41; lean_object* x_42; lean_object* x_43; lean_object* x_44; lean_object* x_45; lean_object* x_46; lean_object* x_47; 
+x_36 = lean_ctor_get(x_24, 0);
+x_37 = lean_ctor_get(x_24, 1);
+lean_inc(x_37);
+lean_inc(x_36);
+lean_dec(x_24);
+x_38 = l_prover_term___u2286_____closed__3;
+x_39 = lean_alloc_ctor(2, 2, 0);
+lean_ctor_set(x_39, 0, x_36);
+lean_ctor_set(x_39, 1, x_38);
+x_40 = l_prover___aux__Src__Prover__Set______unexpand__prover__mem__1___closed__3;
+x_41 = lean_array_push(x_40, x_21);
+x_42 = lean_array_push(x_41, x_39);
+x_43 = lean_array_push(x_42, x_22);
+x_44 = lean_box(2);
+x_45 = l_prover_term___u2286_____closed__2;
+x_46 = lean_alloc_ctor(1, 3, 0);
+lean_ctor_set(x_46, 0, x_44);
+lean_ctor_set(x_46, 1, x_45);
+lean_ctor_set(x_46, 2, x_43);
+x_47 = lean_alloc_ctor(0, 2, 0);
+lean_ctor_set(x_47, 0, x_46);
+lean_ctor_set(x_47, 1, x_37);
+return x_47;
+}
+}
+}
+}
+}
+}
+LEAN_EXPORT lean_object* l_prover___aux__Src__Prover__Set______unexpand__prover__subset__1___boxed(lean_object* x_1, lean_object* x_2, lean_object* x_3) {
+_start:
+{
+lean_object* x_4; 
+x_4 = l_prover___aux__Src__Prover__Set______unexpand__prover__subset__1(x_1, x_2, x_3);
+lean_dec(x_2);
+return x_4;
+}
+}
+lean_object* initialize_Init(uint8_t builtin, lean_object*);
+lean_object* initialize_Src_Prover_Choice(uint8_t builtin, lean_object*);
+static bool _G_initialized = false;
+LEAN_EXPORT lean_object* initialize_Src_Prover_Set(uint8_t builtin, lean_object* w) {
+lean_object * res;
+if (_G_initialized) return lean_io_result_mk_ok(lean_box(0));
+_G_initialized = true;
+res = initialize_Init(builtin, lean_io_mk_world());
+if (lean_io_result_is_error(res)) return res;
+lean_dec_ref(res);
+res = initialize_Src_Prover_Choice(builtin, lean_io_mk_world());
+if (lean_io_result_is_error(res)) return res;
+lean_dec_ref(res);
+l_prover_term___u2208_____closed__1 = _init_l_prover_term___u2208_____closed__1();
+lean_mark_persistent(l_prover_term___u2208_____closed__1);
+l_prover_term___u2208_____closed__2 = _init_l_prover_term___u2208_____closed__2();
+lean_mark_persistent(l_prover_term___u2208_____closed__2);
+l_prover_term___u2208_____closed__3 = _init_l_prover_term___u2208_____closed__3();
+lean_mark_persistent(l_prover_term___u2208_____closed__3);
+l_prover_term___u2208_____closed__4 = _init_l_prover_term___u2208_____closed__4();
+lean_mark_persistent(l_prover_term___u2208_____closed__4);
+l_prover_term___u2208_____closed__5 = _init_l_prover_term___u2208_____closed__5();
+lean_mark_persistent(l_prover_term___u2208_____closed__5);
+l_prover_term___u2208_____closed__6 = _init_l_prover_term___u2208_____closed__6();
+lean_mark_persistent(l_prover_term___u2208_____closed__6);
+l_prover_term___u2208_____closed__7 = _init_l_prover_term___u2208_____closed__7();
+lean_mark_persistent(l_prover_term___u2208_____closed__7);
+l_prover_term___u2208_____closed__8 = _init_l_prover_term___u2208_____closed__8();
+lean_mark_persistent(l_prover_term___u2208_____closed__8);
+l_prover_term___u2208_____closed__9 = _init_l_prover_term___u2208_____closed__9();
+lean_mark_persistent(l_prover_term___u2208_____closed__9);
+l_prover_term___u2208_____closed__10 = _init_l_prover_term___u2208_____closed__10();
+lean_mark_persistent(l_prover_term___u2208_____closed__10);
+l_prover_term___u2208_____closed__11 = _init_l_prover_term___u2208_____closed__11();
+lean_mark_persistent(l_prover_term___u2208_____closed__11);
+l_prover_term___u2208_____closed__12 = _init_l_prover_term___u2208_____closed__12();
+lean_mark_persistent(l_prover_term___u2208_____closed__12);
+l_prover_term___u2208_____closed__13 = _init_l_prover_term___u2208_____closed__13();
+lean_mark_persistent(l_prover_term___u2208_____closed__13);
+l_prover_term___u2208__ = _init_l_prover_term___u2208__();
+lean_mark_persistent(l_prover_term___u2208__);
+l_prover___aux__Src__Prover__Set______macroRules__prover__term___u2208____1___closed__1 = _init_l_prover___aux__Src__Prover__Set______macroRules__prover__term___u2208____1___closed__1();
+lean_mark_persistent(l_prover___aux__Src__Prover__Set______macroRules__prover__term___u2208____1___closed__1);
+l_prover___aux__Src__Prover__Set______macroRules__prover__term___u2208____1___closed__2 = _init_l_prover___aux__Src__Prover__Set______macroRules__prover__term___u2208____1___closed__2();
+lean_mark_persistent(l_prover___aux__Src__Prover__Set______macroRules__prover__term___u2208____1___closed__2);
+l_prover___aux__Src__Prover__Set______macroRules__prover__term___u2208____1___closed__3 = _init_l_prover___aux__Src__Prover__Set______macroRules__prover__term___u2208____1___closed__3();
+lean_mark_persistent(l_prover___aux__Src__Prover__Set______macroRules__prover__term___u2208____1___closed__3);
+l_prover___aux__Src__Prover__Set______macroRules__prover__term___u2208____1___closed__4 = _init_l_prover___aux__Src__Prover__Set______macroRules__prover__term___u2208____1___closed__4();
+lean_mark_persistent(l_prover___aux__Src__Prover__Set______macroRules__prover__term___u2208____1___closed__4);
+l_prover___aux__Src__Prover__Set______macroRules__prover__term___u2208____1___closed__5 = _init_l_prover___aux__Src__Prover__Set______macroRules__prover__term___u2208____1___closed__5();
+lean_mark_persistent(l_prover___aux__Src__Prover__Set______macroRules__prover__term___u2208____1___closed__5);
+l_prover___aux__Src__Prover__Set______macroRules__prover__term___u2208____1___closed__6 = _init_l_prover___aux__Src__Prover__Set______macroRules__prover__term___u2208____1___closed__6();
+lean_mark_persistent(l_prover___aux__Src__Prover__Set______macroRules__prover__term___u2208____1___closed__6);
+l_prover___aux__Src__Prover__Set______macroRules__prover__term___u2208____1___closed__7 = _init_l_prover___aux__Src__Prover__Set______macroRules__prover__term___u2208____1___closed__7();
+lean_mark_persistent(l_prover___aux__Src__Prover__Set______macroRules__prover__term___u2208____1___closed__7);
+l_prover___aux__Src__Prover__Set______macroRules__prover__term___u2208____1___closed__8 = _init_l_prover___aux__Src__Prover__Set______macroRules__prover__term___u2208____1___closed__8();
+lean_mark_persistent(l_prover___aux__Src__Prover__Set______macroRules__prover__term___u2208____1___closed__8);
+l_prover___aux__Src__Prover__Set______macroRules__prover__term___u2208____1___closed__9 = _init_l_prover___aux__Src__Prover__Set______macroRules__prover__term___u2208____1___closed__9();
+lean_mark_persistent(l_prover___aux__Src__Prover__Set______macroRules__prover__term___u2208____1___closed__9);
+l_prover___aux__Src__Prover__Set______macroRules__prover__term___u2208____1___closed__10 = _init_l_prover___aux__Src__Prover__Set______macroRules__prover__term___u2208____1___closed__10();
+lean_mark_persistent(l_prover___aux__Src__Prover__Set______macroRules__prover__term___u2208____1___closed__10);
+l_prover___aux__Src__Prover__Set______macroRules__prover__term___u2208____1___closed__11 = _init_l_prover___aux__Src__Prover__Set______macroRules__prover__term___u2208____1___closed__11();
+lean_mark_persistent(l_prover___aux__Src__Prover__Set______macroRules__prover__term___u2208____1___closed__11);
+l_prover___aux__Src__Prover__Set______macroRules__prover__term___u2208____1___closed__12 = _init_l_prover___aux__Src__Prover__Set______macroRules__prover__term___u2208____1___closed__12();
+lean_mark_persistent(l_prover___aux__Src__Prover__Set______macroRules__prover__term___u2208____1___closed__12);
+l_prover___aux__Src__Prover__Set______macroRules__prover__term___u2208____1___closed__13 = _init_l_prover___aux__Src__Prover__Set______macroRules__prover__term___u2208____1___closed__13();
+lean_mark_persistent(l_prover___aux__Src__Prover__Set______macroRules__prover__term___u2208____1___closed__13);
+l_prover___aux__Src__Prover__Set______macroRules__prover__term___u2208____1___closed__14 = _init_l_prover___aux__Src__Prover__Set______macroRules__prover__term___u2208____1___closed__14();
+lean_mark_persistent(l_prover___aux__Src__Prover__Set______macroRules__prover__term___u2208____1___closed__14);
+l_prover___aux__Src__Prover__Set______macroRules__prover__term___u2208____1___closed__15 = _init_l_prover___aux__Src__Prover__Set______macroRules__prover__term___u2208____1___closed__15();
+lean_mark_persistent(l_prover___aux__Src__Prover__Set______macroRules__prover__term___u2208____1___closed__15);
+l_prover___aux__Src__Prover__Set______macroRules__prover__term___u2208____1___closed__16 = _init_l_prover___aux__Src__Prover__Set______macroRules__prover__term___u2208____1___closed__16();
+lean_mark_persistent(l_prover___aux__Src__Prover__Set______macroRules__prover__term___u2208____1___closed__16);
+l_prover___aux__Src__Prover__Set______macroRules__prover__term___u2208____1___closed__17 = _init_l_prover___aux__Src__Prover__Set______macroRules__prover__term___u2208____1___closed__17();
+lean_mark_persistent(l_prover___aux__Src__Prover__Set______macroRules__prover__term___u2208____1___closed__17);
+l_prover___aux__Src__Prover__Set______macroRules__prover__term___u2208____1___closed__18 = _init_l_prover___aux__Src__Prover__Set______macroRules__prover__term___u2208____1___closed__18();
+lean_mark_persistent(l_prover___aux__Src__Prover__Set______macroRules__prover__term___u2208____1___closed__18);
+l_prover___aux__Src__Prover__Set______unexpand__prover__mem__1___closed__1 = _init_l_prover___aux__Src__Prover__Set______unexpand__prover__mem__1___closed__1();
+lean_mark_persistent(l_prover___aux__Src__Prover__Set______unexpand__prover__mem__1___closed__1);
+l_prover___aux__Src__Prover__Set______unexpand__prover__mem__1___closed__2 = _init_l_prover___aux__Src__Prover__Set______unexpand__prover__mem__1___closed__2();
+lean_mark_persistent(l_prover___aux__Src__Prover__Set______unexpand__prover__mem__1___closed__2);
+l_prover___aux__Src__Prover__Set______unexpand__prover__mem__1___closed__3 = _init_l_prover___aux__Src__Prover__Set______unexpand__prover__mem__1___closed__3();
+lean_mark_persistent(l_prover___aux__Src__Prover__Set______unexpand__prover__mem__1___closed__3);
+l_prover_term___u2209_____closed__1 = _init_l_prover_term___u2209_____closed__1();
+lean_mark_persistent(l_prover_term___u2209_____closed__1);
+l_prover_term___u2209_____closed__2 = _init_l_prover_term___u2209_____closed__2();
+lean_mark_persistent(l_prover_term___u2209_____closed__2);
+l_prover_term___u2209_____closed__3 = _init_l_prover_term___u2209_____closed__3();
+lean_mark_persistent(l_prover_term___u2209_____closed__3);
+l_prover_term___u2209_____closed__4 = _init_l_prover_term___u2209_____closed__4();
+lean_mark_persistent(l_prover_term___u2209_____closed__4);
+l_prover_term___u2209_____closed__5 = _init_l_prover_term___u2209_____closed__5();
+lean_mark_persistent(l_prover_term___u2209_____closed__5);
+l_prover_term___u2209_____closed__6 = _init_l_prover_term___u2209_____closed__6();
+lean_mark_persistent(l_prover_term___u2209_____closed__6);
+l_prover_term___u2209__ = _init_l_prover_term___u2209__();
+lean_mark_persistent(l_prover_term___u2209__);
+l_prover___aux__Src__Prover__Set______macroRules__prover__term___u2209____1___closed__1 = _init_l_prover___aux__Src__Prover__Set______macroRules__prover__term___u2209____1___closed__1();
+lean_mark_persistent(l_prover___aux__Src__Prover__Set______macroRules__prover__term___u2209____1___closed__1);
+l_prover___aux__Src__Prover__Set______macroRules__prover__term___u2209____1___closed__2 = _init_l_prover___aux__Src__Prover__Set______macroRules__prover__term___u2209____1___closed__2();
+lean_mark_persistent(l_prover___aux__Src__Prover__Set______macroRules__prover__term___u2209____1___closed__2);
+l_prover___aux__Src__Prover__Set______macroRules__prover__term___u2209____1___closed__3 = _init_l_prover___aux__Src__Prover__Set______macroRules__prover__term___u2209____1___closed__3();
+lean_mark_persistent(l_prover___aux__Src__Prover__Set______macroRules__prover__term___u2209____1___closed__3);
+l_prover___aux__Src__Prover__Set______macroRules__prover__term___u2209____1___closed__4 = _init_l_prover___aux__Src__Prover__Set______macroRules__prover__term___u2209____1___closed__4();
+lean_mark_persistent(l_prover___aux__Src__Prover__Set______macroRules__prover__term___u2209____1___closed__4);
+l_prover___aux__Src__Prover__Set______macroRules__prover__term___u2209____1___closed__5 = _init_l_prover___aux__Src__Prover__Set______macroRules__prover__term___u2209____1___closed__5();
+lean_mark_persistent(l_prover___aux__Src__Prover__Set______macroRules__prover__term___u2209____1___closed__5);
+l_prover___aux__Src__Prover__Set______macroRules__prover__term___u2209____1___closed__6 = _init_l_prover___aux__Src__Prover__Set______macroRules__prover__term___u2209____1___closed__6();
+lean_mark_persistent(l_prover___aux__Src__Prover__Set______macroRules__prover__term___u2209____1___closed__6);
+l_prover___aux__Src__Prover__Set______macroRules__prover__term___u2209____1___closed__7 = _init_l_prover___aux__Src__Prover__Set______macroRules__prover__term___u2209____1___closed__7();
+lean_mark_persistent(l_prover___aux__Src__Prover__Set______macroRules__prover__term___u2209____1___closed__7);
+l_prover_term___u2286_____closed__1 = _init_l_prover_term___u2286_____closed__1();
+lean_mark_persistent(l_prover_term___u2286_____closed__1);
+l_prover_term___u2286_____closed__2 = _init_l_prover_term___u2286_____closed__2();
+lean_mark_persistent(l_prover_term___u2286_____closed__2);
+l_prover_term___u2286_____closed__3 = _init_l_prover_term___u2286_____closed__3();
+lean_mark_persistent(l_prover_term___u2286_____closed__3);
+l_prover_term___u2286_____closed__4 = _init_l_prover_term___u2286_____closed__4();
+lean_mark_persistent(l_prover_term___u2286_____closed__4);
+l_prover_term___u2286_____closed__5 = _init_l_prover_term___u2286_____closed__5();
+lean_mark_persistent(l_prover_term___u2286_____closed__5);
+l_prover_term___u2286_____closed__6 = _init_l_prover_term___u2286_____closed__6();
+lean_mark_persistent(l_prover_term___u2286_____closed__6);
+l_prover_term___u2286__ = _init_l_prover_term___u2286__();
+lean_mark_persistent(l_prover_term___u2286__);
+l_prover___aux__Src__Prover__Set______macroRules__prover__term___u2286____1___closed__1 = _init_l_prover___aux__Src__Prover__Set______macroRules__prover__term___u2286____1___closed__1();
+lean_mark_persistent(l_prover___aux__Src__Prover__Set______macroRules__prover__term___u2286____1___closed__1);
+l_prover___aux__Src__Prover__Set______macroRules__prover__term___u2286____1___closed__2 = _init_l_prover___aux__Src__Prover__Set______macroRules__prover__term___u2286____1___closed__2();
+lean_mark_persistent(l_prover___aux__Src__Prover__Set______macroRules__prover__term___u2286____1___closed__2);
+l_prover___aux__Src__Prover__Set______macroRules__prover__term___u2286____1___closed__3 = _init_l_prover___aux__Src__Prover__Set______macroRules__prover__term___u2286____1___closed__3();
+lean_mark_persistent(l_prover___aux__Src__Prover__Set______macroRules__prover__term___u2286____1___closed__3);
+l_prover___aux__Src__Prover__Set______macroRules__prover__term___u2286____1___closed__4 = _init_l_prover___aux__Src__Prover__Set______macroRules__prover__term___u2286____1___closed__4();
+lean_mark_persistent(l_prover___aux__Src__Prover__Set______macroRules__prover__term___u2286____1___closed__4);
+l_prover___aux__Src__Prover__Set______macroRules__prover__term___u2286____1___closed__5 = _init_l_prover___aux__Src__Prover__Set______macroRules__prover__term___u2286____1___closed__5();
+lean_mark_persistent(l_prover___aux__Src__Prover__Set______macroRules__prover__term___u2286____1___closed__5);
+l_prover___aux__Src__Prover__Set______macroRules__prover__term___u2286____1___closed__6 = _init_l_prover___aux__Src__Prover__Set______macroRules__prover__term___u2286____1___closed__6();
+lean_mark_persistent(l_prover___aux__Src__Prover__Set______macroRules__prover__term___u2286____1___closed__6);
+l_prover___aux__Src__Prover__Set______macroRules__prover__term___u2286____1___closed__7 = _init_l_prover___aux__Src__Prover__Set______macroRules__prover__term___u2286____1___closed__7();
+lean_mark_persistent(l_prover___aux__Src__Prover__Set______macroRules__prover__term___u2286____1___closed__7);
+return lean_io_result_mk_ok(lean_box(0));
+}
+#ifdef __cplusplus
+}
+#endif
