Src/prover/Main.lean
@@ -12,7 +12,7 @@ theorem not_mem_of_empty {a b} (h : empty a) : b ∉ a :=
 theorem empty_iff {a} : empty a ↔ ∀ b, b ∉ a :=
 iff_intro (λ h _ => not_mem_of_empty h) (λ h h₁ => exi_elim h₁ h)
 
-theorem nonempty_intro {a b} (h : b ∈ a) : nonempty a :=
+theorem nonempty_intro {a} b (h : b ∈ a) : nonempty a :=
 not_not_intro # exi_intro b h
 
 theorem nonempty_elim {P : Prop} {a} (h₁ : nonempty a) (h₂ : ∀ b, b ∈ a → P) : P :=
@@ -31,3 +31,47 @@ notation (priority := high) "∅" => emp
 
 theorem empty_emp : empty ∅ :=
 some_spec exi_empty
+
+theorem exi_nonempty : ∃ a, nonempty a :=
+exi_elim ax_inf # λ a h₁ => exi_elim h₁ # λ b h₂ => exi_intro a #
+nonempty_intro b # and_left # and_right h₂
+
+def spec (a : Set) (P : Set → Prop) : Set :=
+some # ax_spec a P
+
+theorem mem_spec {a b} {P : Set → Prop} : b ∈ spec a P ↔ b ∈ a ∧ P b :=
+some_spec (ax_spec a P) b
+
+def fun_to_pred {α β : Type} (f : α → β) (x : α) (y : β) : Prop :=
+f x = y
+
+theorem fun_to_pred_iff {α β : Type} {f : α → β} {x : α} {y : β} :
+  fun_to_pred f x y ↔ f x = y :=
+iff_refl
+
+theorem exiu_fun_to_pred {α β : Type} {f : α → β} {x : α} :
+  ∃! (y : β), fun_to_pred f x y :=
+exiu_intro (f x) rfl # λ y h => eq_symm h
+
+def image_aux (a : Set) (f : Set → Set) : Set :=
+some # ax_rep a (fun_to_pred f) # λ b h => exiu_fun_to_pred
+
+theorem mem_image_aux_of {a b : Set} {f : Set → Set}
+  (h : ∃ c, c ∈ a ∧ f c = b) : b ∈ image_aux a f :=
+sorry
+
+#exit
+
+def image (a : Set) (f : Set → Set) : Set :=
+spec (image_aux a f) # λ b => ∃ c, c ∈ a ∧ f c = b
+
+theorem mem_image {a b : Set} {f : Set → Set} :
+  b ∈ image a f ↔ ∃ c, c ∈ a ∧ f c = b :=
+iff_intro
+(λ h => and_right # mp mem_spec h)
+(λ h => mpr mem_spec # and_intro _ h)
+
+#exit
+
+theorem mem_irrefl {a} : a ∉ a :=
+_
