Src/prover/Logic.lean
@@ -262,7 +262,7 @@ iff_intro
 (λ h x h₁ => h # exi_intro x h₁)
 (λ h h₁ => exi_elim h₁ h)
 
-theorem exiu_intro {α : Type} {P : α → Prop} (h₁ : ∃ (x : α), P x)
+theorem exiu_intro' {α : Type} {P : α → Prop} (h₁ : ∃ (x : α), P x)
   (h₂ : ∀ (x y : α), P x → P y → x = y) : ∃! (x : α), P x :=
 and_intro h₁ h₂
 
@@ -339,5 +339,9 @@ theorem exiu_iff {α : Type} {P : α → Prop} :
   (∃! (x : α), P x) ↔ ∃ (x : α), P x ∧ ∀ (y : α), P y → y = x :=
 iff_intro
 (λ h => exiu_elim h # λ x h₁ h₂ => exi_intro x # and_intro h₁ h₂)
-(λ h => exi_elim h # λ x h₁ => exiu_intro (exi_intro x # and_left h₁)
+(λ h => exi_elim h # λ x h₁ => exiu_intro' (exi_intro x # and_left h₁)
   (λ y z h₃ h₄ => and_elim h₁ # λ h₅ h₆ => eq_trans x (h₆ y h₃) # eq_symm # h₆ z h₄))
+
+theorem exiu_intro {α : Type} {P : α → Prop} (x : α)
+  (h₁ : P x) (h₂ : ∀ (y : α), P y → y = x) : ∃! (x : α), P x :=
+mpr exiu_iff # exi_intro x # and_intro h₁ h₂
