Src/prover/Set.lean
@@ -33,9 +33,9 @@ infix:50 (priority := high) " ⊆ " => subset
 
 axiom ax_ext {a b} : (∀ c, c ∈ a ↔ c ∈ b) → a = b
 axiom ax_reg {a} : nonempty a → ∃ b, b ∈ a ∧ ¬∃ c, c ∈ b ∧ c ∈ a
-axiom ax_spec (P : Set → Prop) a : ∃ b, ∀ c, c ∈ b ↔ c ∈ a ∧ P c
+axiom ax_spec a (P : Set → Prop) : ∃ b, ∀ c, c ∈ b ↔ c ∈ a ∧ P c
 axiom ax_union a : ∃ b, ∀ c d, (d ∈ c ∧ c ∈ a) → d ∈ b
-axiom ax_rep (P : Set → Set → Prop) {a} : (∀ b, b ∈ a → ∃! c, P b c) →
+axiom ax_rep a (P : Set → Set → Prop) : (∀ b, b ∈ a → ∃! c, P b c) →
   ∃ b, ∀ c, c ∈ a → ∃ d, d ∈ b ∧ P c d
 axiom ax_inf : ∃ a b, empty b ∧ b ∈ a ∧ ∀ c, c ∈ a → ∀ d, is_set_succ c d → d ∈ a
 axiom ax_pow : ∀ a, ∃ b, ∀ c, c ⊆ a → c ∈ b
